read_device

proofs/inv_read.dfy
@@ -24,13 +24,45 @@ method dma_read(vpn : int,
 
     // The data is unchanged
     ensures host_tlb[vpn].ppn in new_host_mem
-    ensures device_tlb[vpn].ppn in device_mem
+    // ensures device_tlb[vpn].ppn in device_mem
     ensures new_host_mem[host_tlb[vpn].ppn] == device_mem[device_tlb[vpn].ppn]
 {
     new_host_mem := host_mem;
     var device_entry := device_tlb[vpn];
 
     new_host_mem := new_host_mem[host_tlb[vpn].ppn := device_mem[device_entry.ppn]];
+}
+
+
+// copies data from host to device
+method dma_write(vpn : int, 
+                host_mem : map<int, page>, host_tlb : map<int, tlb_entry>, 
+                device_mem : map<int, page>, device_tlb : map<int, tlb_entry>)
+
+    returns (new_device_mem : map<int, page>)
+
+    // There must be a tlb entry and ppn dedicated on the host
+    // Our DMA transfer method also requires the vpn to be writeable
+    requires vpn in host_tlb
+    requires legal_vaddr(vpn, host_mem, host_tlb)
+
+    // We are reading from the device, there should be data there
+    requires(vpn_present(vpn, device_mem, device_tlb))
+
+
+    // Original host/device pages are untouched
+    ensures no_side_effects(vpn, device_mem, device_tlb, new_device_mem, device_tlb)
+    ensures valid_ppns(device_mem, device_tlb) ==> valid_ppns(new_device_mem, device_tlb)
+    ensures valid_memory(host_mem, host_tlb, device_mem, device_tlb) ==> valid_memory(host_mem, host_tlb, new_device_mem, device_tlb)
+
+    // The data is unchanged
+    ensures device_tlb[vpn].ppn in new_device_mem
+    ensures new_device_mem[device_tlb[vpn].ppn] == host_mem[host_tlb[vpn].ppn]
+{
+    new_device_mem := device_mem;
+    var host_entry := host_tlb[vpn];
+
+    new_device_mem := new_device_mem[device_tlb[vpn].ppn := host_mem[host_entry.ppn]];
 }
 
 method write_tlb(vpn : int, ppn : int, present : bool, readable : bool, writable : bool, tlb : map<int, tlb_entry>, ghost mem : map<int, page>, ghost other_tlb : map<int, tlb_entry>, ghost other_mem : map<int, page>)
@@ -97,21 +129,34 @@ function no_side_effects(vpn : int, mem : map<int, page>, tlb : map<int, tlb_ent
 function data_unchanged(vpn : int, host_mem : map<int, page>, host_tlb : map<int, tlb_entry>, device_mem : map<int, page>, device_tlb : map<int, tlb_entry>, data : int, 
             new_host_mem : map<int, page>, new_host_tlb : map<int, tlb_entry>, 
             new_device_mem : map<int, page>, new_device_tlb : map<int, tlb_entry>) : bool
-            requires vpn in new_host_tlb
+            requires vpn_present(vpn, new_host_mem, new_host_tlb) || vpn_present(vpn, new_device_mem, new_device_tlb)
+            requires vpn_present(vpn, host_mem, host_tlb) || vpn_present(vpn, device_mem, device_tlb)
 {
-    (vpn_present(vpn, host_mem, host_tlb) ==> data == host_mem[host_tlb[vpn].ppn].data) &&
-    (vpn_present(vpn, device_mem, device_tlb) ==> data == device_mem[device_tlb[vpn].ppn].data)
+    var saved_data := if vpn_present(vpn, new_host_mem, new_host_tlb) then 
+        new_host_mem[new_host_tlb[vpn].ppn].data
+    else 
+        new_device_mem[new_device_tlb[vpn].ppn].data;
+
+    var original_data := if vpn_present(vpn, host_mem, host_tlb) then
+        host_mem[host_tlb[vpn].ppn].data
+    else
+        device_mem[device_tlb[vpn].ppn].data;
+    
+    saved_data == data && saved_data == original_data
 }
 
 function permissions_unchanged(vpn : int, host_mem : map<int, page>, host_tlb : map<int, tlb_entry>, device_mem : map<int, page>, device_tlb : map<int, tlb_entry>, data : int, 
             new_host_mem : map<int, page>, new_host_tlb : map<int, tlb_entry>, 
             new_device_mem : map<int, page>, new_device_tlb : map<int, tlb_entry>) : bool
-            requires vpn in new_host_tlb
+            // requires vpn_present(vpn, new_host_mem, new_host_tlb) || vpn_present(vpn, new_device_mem, new_device_tlb)
+            // requires vpn_present(vpn, host_mem, host_tlb) || vpn_present(vpn, device_mem, device_tlb)
 {
     // The permissions must be unchanged
-    (vpn_present(vpn, host_mem, host_tlb) ==> new_host_tlb[vpn] == host_tlb[vpn]) &&
-    (vpn_present(vpn, device_mem, device_tlb) ==> new_host_tlb[vpn].readable == device_tlb[vpn].readable) &&
-    (vpn_present(vpn, device_mem, device_tlb) ==> new_host_tlb[vpn].writable == device_tlb[vpn].writable)
+    (vpn_present(vpn, host_mem, host_tlb) && vpn_present(vpn, new_host_mem, new_host_tlb) ==> new_host_tlb[vpn] == host_tlb[vpn]) &&
+    (vpn_present(vpn, device_mem, device_tlb) && vpn_present(vpn, new_host_mem, new_host_tlb) ==> (new_host_tlb[vpn].readable == device_tlb[vpn].readable) && new_host_tlb[vpn].writable == device_tlb[vpn].writable) &&
+
+    (vpn_present(vpn, device_mem, device_tlb) && vpn_present(vpn, new_device_mem, new_device_tlb) ==> new_device_tlb[vpn] == device_tlb[vpn]) &&
+    (vpn_present(vpn, host_mem, host_tlb) && vpn_present(vpn, new_device_mem, new_device_tlb) ==> (host_tlb[vpn].readable == new_device_tlb[vpn].readable) && host_tlb[vpn].writable == new_device_tlb[vpn].writable)
 }
 
 function valid_ppns(mem : map<int, page>, tlb : map<int, tlb_entry>) : bool 
@@ -224,4 +269,78 @@ method write_host(vpn : int, data : int,
     }
     new_host_mem := new_host_mem[new_host_tlb[vpn].ppn := page.Node(data)];
     return; 
+}
+
+method allocate_device_ppn(device_mem : map<int, page>)
+    returns (pg : int, new_device_mem : map<int, page>)
+    ensures pg !in device_mem
+    ensures pg in new_device_mem
+    ensures forall p :: p in device_mem ==> p in new_device_mem && device_mem[p] == new_device_mem[p]
+{
+    var keys := device_mem.Keys;
+    pg := 0;
+    var seen := {};
+    while keys != {} 
+        invariant |seen| > 0 ==> forall k :: k in seen ==> pg > k
+        invariant forall k :: k in device_mem.Keys ==> k in seen || k in keys
+    {
+        var key :| key in keys;
+        keys := keys - {key};
+        seen := seen + {key};
+
+        if key >= pg {
+            pg := key + 1;
+        }
+    }
+
+    new_device_mem := device_mem[pg := page.Node(0)];
+}
+
+// read from memory on the device
+method read_device(vpn : int, 
+                host_mem : map<int, page>, host_tlb : map<int, tlb_entry>, 
+                device_mem : map<int, page>, device_tlb : map<int, tlb_entry>)
+
+    returns (data : int, 
+            new_host_mem : map<int, page>, new_host_tlb : map<int, tlb_entry>, 
+            new_device_mem : map<int, page>, new_device_tlb : map<int, tlb_entry>)
+
+    // data must exist on the host so that we have a ppn for it
+    requires legal_vaddr(vpn, host_mem, host_tlb)
+    // Data must also exist and be readable somewhere
+    requires ppn_readable(vpn, host_mem, host_tlb) || ppn_readable(vpn, device_mem, device_tlb)
+    requires valid_memory(host_mem, host_tlb, device_mem, device_tlb)
+
+    // ensures vpn_present(vpn, new_host_mem, new_host_tlb)
+    // The data should reside on the device after executing this method
+    ensures ppn_readable(vpn, new_device_mem, new_device_tlb)
+
+    // The data should not be accessible on the host after executing this method
+    ensures !vpn_present(vpn, new_host_mem, new_host_tlb)
+
+    ensures data_unchanged(vpn, host_mem, host_tlb, device_mem, device_tlb, data, new_host_mem, new_host_tlb, new_device_mem, new_device_tlb)
+
+    // pages other than vpn are not changed in any way
+    ensures no_side_effects(vpn, host_mem, host_tlb, new_host_mem, new_host_tlb)
+    ensures no_side_effects(vpn, device_mem, device_tlb, device_mem, new_device_tlb)
+
+    ensures permissions_unchanged(vpn, host_mem, host_tlb, device_mem, device_tlb, data, new_host_mem, new_host_tlb, device_mem, new_device_tlb)
+    ensures valid_memory(new_host_mem, new_host_tlb, new_device_mem, new_device_tlb)
+{
+    new_host_mem := host_mem;
+    new_host_tlb := host_tlb;
+
+    new_device_mem := device_mem;
+    new_device_tlb := device_tlb;
+
+    if vpn !in device_tlb || !device_tlb[vpn].present {
+        var should_be_writable := host_tlb[vpn].writable;
+        var ppn;
+        ppn, new_device_mem := allocate_device_ppn(device_mem);
+        new_host_tlb := write_tlb(vpn, 0, false, false, false, host_tlb, new_host_mem, new_device_tlb, new_device_mem);
+        new_device_tlb := write_tlb(vpn, ppn, true, true, should_be_writable, new_device_tlb, new_device_mem, new_host_tlb, new_host_mem);
+        new_device_mem := dma_write(vpn, host_mem, host_tlb, new_device_mem, new_device_tlb);
+    } 
+    data := new_device_mem[new_device_tlb[vpn].ppn].data;
+    return;
 }
